\documentclass{article}
\usepackage{amsmath}
\begin{document}
\begin{itemize}
\item Convection/Diffusion
\item Hyperbolic
\item Numerical Integration
\item Interpolation
\item Parallel computing
\end{itemize}
\renewcommand{\d}[2]{\frac{\partial #1}{\partial #2}}
\newcommand{\dtwo}[2]{\frac{\partial^2 #1}{\partial #2^2}}
\begin{align}
  \theta_t + + u \theta_x = \Gamma \theta_{xx} \\
  \d{\theta}{t} + u \d{\theta}{x} = \Gamma\dtwo{\theta}{x} \\
  \text{let }\varphi = \rho Y_i \\
  \d{\rho Y_i}{t} + \vec{v}\cdot \nabla \rho Y_i = \rho \Gamma \nabla^2 Y_i
  \nabla \cdot \vec{v} = 0
\end{align}
FTCS
\begin{align}
  \varphi^{n+1} = \varphi^n - \frac{u\Delta t}{z\Delta x}\left(\varphi_{i+1}-\varphi_{i-1}\right)^n + \frac{\Gamma \Delta t}{\Delta x^2}\left(\varphi_{i+1}-2\varphi_{i}+\varphi_{i-1}\right)
  \label{FTCS}
\end{align}

SS.
\begin{align}
  \d{u\phi}{x} = \Gamma \dtwo{\phi}{x}\\
  (u\phi)_e - (u\phi)_w = \Gamma \left(\d{\phi}{x}\right)_e - \Gamma \left(\d{\phi}{x}\right)_w\\
  \frac{1}{2}u_e\left(\phi_E + \phi_P\right) - \frac{1}{2}u_w\left(\phi_P + \phi_W\right) = \frac{\Gamma}{\delta}\left(\phi_E - \phi_P\right) - \frac{\Gamma}{\delta}\left(\phi_P - \phi_W\right)\\
  %\phi_W\left[-\frac{1]{2}u - \frac{\Gamma}{\delta}\right] + \phi_P\left[2\Gamma}{\delta}\right] + \phi_E\left[\frac{1}{2}u-\frac{\Gamma}{\delta}\right]=0\\
  Re = \frac{u\delta}{\Gamma}\\
  \phi_W\left[-\frac{Re}{2}-1\right]+\phi_P\left[2\right] + \phi_E\left[\frac{Re}{2}-1\right] = 0\\
  \phi_P = \frac{1}{2} \left[\phi_w\left(\frac{Re}{2} + 1\right) - \phi_E\left(\frac{Re}{2} - 1\right)\right]
  \label{Why FTCS is wrong for convective}
\end{align}
FTCS is wrong for this example for two reasons:
\begin{itemize}
  \item Unphysical results can occur
  \item Dependent on Reynold's number
\end{itemize}
$c_p \phi_p = c_E\phi_E + c_W\phi_W$
Mass balance is 
\begin{align}
\d{\rho}{t} + \d{u}{x} = 0\\
\d{u}{x} = 0
\end{align}

Add Upwinding
let $u>0$
\begin{align}
  u\phi_e - u\phi_w = \Gamma (\d{\phi}{x})_e - \Gamma(\d{\phi}{x})_w\\
  u\phi_p - u\phi_W = \Gamma(\phi_E - \phi_P) - \frac{\Gamma}{\delta}(\phi_p-\phi_w)\\
  \phi_p = \phi_E\left[(\frac{\Gamma}{\delta})/(u + 2 \frac{\Gamma}{\delta})\right] + \phi_W\left[(u+\frac{\Gamma}{\delta})/(u + 2 \frac{\Gamma}{\delta})\right] 
  \label{Upwinding}
\end{align}
\end{document}
